Final stint

theories/AL/AL.v
@@ -1,13 +1,13 @@
 From Stdlib Require Export NArith String.
 From ILAL Require Export AL.language state tactics.
 From Stdlib Require Import List.
+From Stdlib Require Import Lia PeanoNat.
 Import ListNotations.
 Open Scope N_scope.
 Open Scope string_scope.
 
 (** Denotational Relational Semantics *)
 (* Table 8 *)
-
 Declare Scope al_ds_scope.
 Open Scope al_ds_scope.
 
@@ -49,6 +49,32 @@ Definition mode_chan_upd (m : mode) (sig : estate) (k : id) (l : channel) : esta
   | Ad => sig[[ k :=ach l ]]
   end.
 
+Lemma mode_upd_shadow : forall m sig x v v',
+  mode_upd m (mode_upd m sig x v) x v' = mode_upd m sig x v'.
+Proof.
+  intros m ((vs & vc) & (as_ & ac)) x v v'. destruct m; simpl;
+    unfold update_victim, update_adversary; simpl;
+    now rewrite update_shadow.
+Qed.
+
+Lemma mode_store_upd_eq : forall m sig x v,
+  mode_store m (mode_upd m sig x v) x = v.
+Proof.
+  intros m ((vs & vc) & (as_ & ac)) x v. destruct m; simpl; now rewrite update_eq.
+Qed.
+
+Lemma mode_upd_store_eq : forall m sig x,
+  mode_upd m sig x (mode_store m sig x) = sig.
+Proof.
+  intros m ((vs & vc) & (as_ & ac)) x. destruct m; simpl;
+    unfold update_victim, update_adversary; simpl; f_equal; f_equal;
+    now rewrite state_upd_eq.
+Qed.
+
+(** Single-thread semantics
+
+    [ [[ c ]] m |=> (s, s') ] : running command [c] in mode [m] can take the
+    single [estate] [s] to [s']. *)
 Inductive ds : astmt -> mode -> (estate * estate) -> Prop :=
 | EDSkip m (s : estate) :
     [[ skip ]] m |=> (s, s)
@@ -102,24 +128,30 @@ Inductive ds : astmt -> mode -> (estate * estate) -> Prop :=
     [[ c** ]] m |=> (s1, s2) ->
     [[ c ]] m |=> (s2, s3) ->
     [[ c** ]] m |=> (s1, s3)
-(** c1 || c2 *)
+(** C1 || C2: parallel composition for independent reduction *)
 | EDParL c1 c2 m s1 s2 :
     [[ c1 ]] m |=> (s1, s2) ->
     [[ c1 <||> c2 ]] m |=> (s1, s2)
 | EDParR c1 c2 m s1 s2 :
     [[ c2 ]] m |=> (s1, s2) ->
     [[ c1 <||> c2 ]] m |=> (s1, s2)
-(** Com(c1, c2) *)
-| EDComVA c1 c2 m ch_id sig v l :
-    sig.(vstate).(ch) ch_id = v :: l ->
-    [[ Com(c1, c2) ]] m |=> (sig, sig[[ch_id :=vch l]][[ch_id :=ach v :: l]])
-| EDComAV c1 c2 m ch_id sig v l :
-    sig.(astate).(ch) ch_id = v :: l ->
-    [[ Com(c1, c2) ]] m |=> (sig, sig[[ch_id :=ach l]][[ch_id :=vch v :: l]])
+(** Com(c1, c2): move the head [v] of the sender's channel to the tail of the receiver's *)
+| EDComVA c1 c2 m ch_id sig v l1 l2 :
+    sig.(vstate).(ch) ch_id = v :: l1 ->
+    sig.(astate).(ch) ch_id = l2 ->
+    [[ Com(c1, c2) ]] m |=>
+      (sig, sig[[ch_id :=vch l1]] [[ch_id :=ach (l2 ++ [v])%list]])
+| EDComAV c1 c2 m ch_id sig v l1 l2 :
+    sig.(astate).(ch) ch_id = v :: l1 ->
+    sig.(vstate).(ch) ch_id = l2 ->
+    [[ Com(c1, c2) ]] m |=>
+      (sig, sig[[ch_id :=ach l1]] [[ch_id :=vch (l2 ++ [v])%list]])
+| EDLocal x e c m sig sig' (x_out : N) :
+    [[ c ]] m |=> (mode_upd m sig x (e (mode_store m sig)), sig') ->
+    [[ local x = e in c ]] m |=>
+      (sig, mode_upd m sig' x x_out)
 where "[[ c ]] m |=> ( s , s' )" := (ds c m (s, s')).
 Close Scope al_scope.
-
-(* Definition 1 *)
 
 Definition post (R : evaluation) (P : aprop) :=
   fun s' => exists s, P s /\ R (s, s').
@@ -138,7 +170,8 @@ Notation "<| P |> c [[ m ]] <| Q |>" :=
   (over_approximate P c m Q)
   (at level 0, c custom al_stmt at level 99, m constr) : al_scope.
 
-(** Lifting predicates into adversarial predicates  *)
+Section PredicateCombinators.
+
 Definition lift (m : mode) (B : prop) : aprop :=
   fun sig => B (mode_store m sig).
 
@@ -155,27 +188,11 @@ Definition anot (P : aprop) : aprop :=
 Definition aand_lift (m : mode) (P : aprop) (B : prop) : aprop :=
   aand P (lift m B).
 
-(** Definition 2 *)
-
-Definition aprop2 : Type := estate -> estate -> Prop.
-
-Definition al_post2 (c1 c2 : astmt) (P A : aprop) : aprop2 :=
-  fun sq sb =>
-    exists sp sa, P sp /\ A sa /\
-      ds c1 Ok (sp, sq) /\ ds c2 Ad (sa, sb).
-
-(* The under-approximate adversarial triple [p][a] c1 || c2 [q][b] *)
-Definition al_under2 (P A : aprop) (c1 c2 : astmt) (Q B : aprop) : Prop :=
-  forall sq sb, Q sq /\ B sb ->
-    al_post2 c1 c2 P A sq sb.
-
-Notation "<[[ P ]][[ A ]] c1 || c2 [[ Q ]][[ B ]]>" :=
-  (al_under2 P A c1 c2 Q B)
-  (at level 0, c1 custom al_stmt at level 99, c2 custom al_stmt at level 99) : al_scope.
+End PredicateCombinators.
 
 Open Scope al_scope.
 
-(** Definition 3 *)
+Section Tier1MetaTheorems.
 
 Theorem and_or_symmetry : forall P Q1 Q2 c m,
   ({{ P }} c [[m]] {{ Q1 }} /\ {{ P }} c [[m]] {{ Q2 }}) <->
@@ -222,11 +239,30 @@ Proof.
   eapply HO. exists s'. auto.
 Qed.
 
-(** Lemma 1 *)
+End Tier1MetaTheorems.
+
+(** Composed, independent triples *)
+
+Definition aprop2 : Type := estate -> estate -> Prop.
+
+Definition al_post2 (c1 c2 : astmt) (P A : aprop) : aprop2 :=
+  fun sq sb =>
+    exists sp sa, P sp /\ A sa /\
+      ds c1 Ok (sp, sq) /\ ds c2 Ad (sa, sb).
+
+(* The under-approximate adversarial triple [p][a] c1 || c2 [q][b] *)
+Definition al_under2 (P A : aprop) (c1 c2 : astmt) (Q B : aprop) : Prop :=
+  forall sq sb, Q sq /\ B sb ->
+    al_post2 c1 c2 P A sq sb.
+
+Notation "'<[[' P ']]' '[[' A ']]' c1 '||' c2 '[[' Q ']]' '[[' B ']]>'" :=
+  (al_under2 P A c1 c2 Q B)
+  (at level 0, c1 custom al_stmt at level 99, c2 custom al_stmt at level 99,
+  format "<[[  P  ]] [[  A  ]]  c1  ||  c2  [[  Q  ]] [[  B  ]]>") : al_scope.
 
 Lemma characterization :
   forall P Q A B C1 C2,
-  <[[P]][[A]] C1 || C2 [[Q]][[B]]> <->
+  <[[P]] [[A]] C1 || C2 [[Q]] [[B]]> <->
   (forall sq sb, Q sq -> B sb ->
     exists sp sa, P sp /\ A sa /\
      ds C1 Ok (sp, sq) /\ ds C2 Ad (sa, sb)).
@@ -238,9 +274,7 @@ Proof.
     exists sq', sb'. auto.
 Qed.
 
-(** Proof rules *)
-(* Page 9 *)
-
+(** Single-threaded Hoare-style proof rules *)
 Reserved Notation
          "P , [ c ] m , Q"
          (at level 40, c custom al_stmt at level 99, P constr, Q constr).
@@ -311,62 +345,26 @@ Inductive derivable : aprop -> astmt -> mode -> aprop -> Prop :=
        (fun sig => exists l,
             P (mode_chan_upd m sig s l)
             /\ mode_chan m sig s = l ++ [mode_store m sig x])%list
-(* Adversarial assertion, success branch *)
+(* Adversarial assertion *)
 | DAdvAssertSuccess : forall Q B,
     Q, [adv_assert(B)] Ad, (aand_lift Ad Q B)
-(* Adversarial assertion, failure branch *)
 | DAdvAssertFailure : forall Q B,
     Q, [adv_assert(B)] Ad, (aand Q (anot (lift Ad B)))
+(* Locals *)
+| DLocal : forall P Q x (e : expression) m c,
+    (fun sig => P (mode_upd m sig x (e (mode_store m sig)))
+                /\ mode_store m sig x = e (mode_store m sig)),
+      [c] m, Q ->
+    P, [local x = e in c] m,
+       (fun sig => exists (sb : estate) (x0 : N),
+            Q sb /\ sig = mode_upd m sb x x0)
 where "P , [ c ] m , Q" := (derivable P c m Q).
-
-Definition denote (c : astmt) (m : mode) : evaluation :=
-  fun '(s1, s2) => [[ c ]] m |=> (s1, s2).
-
-Definition interpret_spec (P Q : aprop) (c : astmt) m : Prop :=
-  P, [c] m, Q <-> {{P}} c [[m]] {{Q}}.
-
-Fixpoint nRepeat (c : astmt) (n : nat) : astmt :=
-  match n with
-  | O => ASkip
-  | S n' => ASeq (nRepeat c n') c
-  end.
 
 Lemma star_equiv : forall c m s1 s2,
   [[ c** ;; c ]] m |=> (s1, s2) ->
   [[ c** ]] m |=> (s1, s2).
 Proof.
   intros c m s1 s2 H. invs H. econstructor; eassumption.
-Qed.
-
-Lemma nRepeat_star : forall c m n s1 s2,
-  ds (nRepeat c n) m (s1, s2) ->
-  [[ c** ]] m |=> (s1, s2).
-Proof.
-  intros c m n. induction n; intros s1 s2 H.
-  - simpl in H. invs H. constructor.
-  - simpl in H. invs H. econstructor; eauto.
-Qed.
-
-(* Conversely, every star execution is some finite [n]-fold repetition *)
-Lemma star_nRepeat : forall c m s1 s2,
-  [[ c** ]] m |=> (s1, s2) ->
-  exists n, ds (nRepeat c n) m (s1, s2).
-Proof.
-  intros c m s1 s2 H.
-  remember <{ c** }> as cs eqn:E.
-  induction H; invs E.
-  - exists O. constructor.
-  - destruct (IHds1 eq_refl) as (n & Hn).
-    exists (S n). econstructor; eauto.
-Qed.
-
-Lemma repeat_is_star : forall c m P s,
-  post (denote <{ c** }> m) P s ->
-  exists n, post (denote (nRepeat c n) m) P s.
-Proof.
-  intros c m P s (s' & Ps' & DS). unfold denote in DS.
-  apply star_nRepeat in DS. destruct DS as (n & Hn).
-  exists n, s'. now split.
 Qed.
 
 Lemma step_assign_ok : forall sig x (e : expression) x',
@@ -501,6 +499,7 @@ Proof.
   unfold update_achannel. simpl. rewrite E. apply EDWriteA.
 Qed.
 
+(* individual thread rule soundness *)
 Theorem soundness :
   forall c P Q m,
     P, [c] m, Q ->
@@ -565,4 +564,994 @@ Proof.
     exists sig. auto using EDAdvAssertSuccess.
   - (* DAdvAssertFailure *) intros sig (Qsig & nBsig).
     exists sig. auto using EDAdvAssertFailure.
+  - (* DLocal *) intros sig (sb & x0 & Qsb & Hsig).
+    destruct (IHderivable sb Qsb) as (sp & (Psp & Hsp_x) & DSbody).
+    assert (Hsp_entry : mode_upd m sp x (e (mode_store m sp)) = sp).
+    { rewrite <- Hsp_x. now rewrite mode_upd_store_eq. }
+    exists sp. split.
+    + rewrite Hsp_entry in Psp. exact Psp.
+    + subst sig.
+      apply (EDLocal x e c m sp sb x0).
+      rewrite Hsp_entry. exact DSbody.
 Qed.
+
+(** Composed semantics and proof system
+
+    The adversarial judgment relates terms [c1] in mode [m1], [c2] in mode [m2],
+    executing in parallel:
+        [m1: P][m2: A]  c1 || c2  [m1: Q][m2: B].
+    Membership of a composed transition [((sp,sa),(sq,sb))] has two cases:
+    1. No interaction between threads
+    2. Victim and adversary step together, sharing information over a channel
+
+    [cds m1 m2 c1 c2 (sp,sa) (sq,sb)] : the composed system [c1||c2] takes one
+    step from [(sp,sa)] to [(sq,sb)] *)
+
+Inductive cds : mode -> mode -> astmt -> astmt ->
+                (estate * estate) -> (estate * estate) -> Prop :=
+(* case 1: independent reduction*)
+| CInd : forall m1 m2 c1 c2 sp sa sq sb,
+    ds c1 m1 (sp, sq) ->
+    ds c2 m2 (sa, sb) ->
+    cds m1 m2 c1 c2 (sp, sa) (sq, sb)
+(* case 2 (Com): a value [v] moves from the head of the program-side channel
+   [s] to the tail of the adversary-side channel [s] *)
+| CComPA : forall m1 m2 c1 c2 (s : id) sp sa v l1 l2,
+    sp.(vstate).(ch) s = v :: l1 ->
+    sa.(astate).(ch) s = l2 ->
+    cds m1 m2 c1 c2 (sp, sa)
+        (sp[[ s :=vch l1 ]], sa[[ s :=ach (l2 ++ [v])%list ]])
+(* vice versa *)
+| CComAP : forall m1 m2 c1 c2 (s : id) sp sa v l1 l2,
+    sa.(astate).(ch) s = v :: l1 ->
+    sp.(vstate).(ch) s = l2 ->
+    cds m1 m2 c1 c2 (sp, sa)
+        (sp[[ s :=vch (l2 ++ [v])%list ]], sa[[ s :=ach l1 ]]).
+
+(* Many steps of [cds], giving the PBV.
+
+   [cds_star m1 m2 c1 c2 p q] : [q] is reachable from [p] by finitely many
+   composed [cds] steps of [c1||c2]. *)
+Inductive cds_star (m1 m2 : mode) (c1 c2 : astmt) :
+  (estate * estate) -> (estate * estate) -> Prop :=
+| CS0 : forall p, cds_star m1 m2 c1 c2 p p
+| CSN : forall p q r,
+    cds_star m1 m2 c1 c2 p q ->
+    cds m1 m2 c1 c2 q r ->
+    cds_star m1 m2 c1 c2 p r.
+
+(** Generalization of [cds_star] to arbitrary [c1,c2] at each
+    step, allowing for proof walkthroughs like we see in the paper *)
+Inductive cds_star_hetero (m1 m2 : mode) :
+  (estate * estate) -> (estate * estate) -> Prop :=
+| CSH0 : forall p, cds_star_hetero m1 m2 p p
+| CSHN : forall c1 c2 p q r,
+    cds_star_hetero m1 m2 p q ->
+    cds m1 m2 c1 c2 q r ->
+    cds_star_hetero m1 m2 p r.
+
+Definition al_postc_star (m1 m2 : mode) (c1 c2 : astmt) (PA : aprop2) : aprop2 :=
+  fun sq sb =>
+    exists sp sa, PA sp sa /\ cds_star m1 m2 c1 c2 (sp, sa) (sq, sb).
+
+Definition al_underc_star (m1 m2 : mode) (PA : aprop2)
+                          (c1 c2 : astmt) (QB : aprop2) : Prop :=
+  forall sq sb, QB sq sb -> al_postc_star m1 m2 c1 c2 PA sq sb.
+
+(** Composed proof system *)
+
+Definition aprod (P A : aprop) : aprop2 := fun sp sa => P sp /\ A sa.
+
+Definition al_postc_r (m1 m2 : mode) (c1 c2 : astmt) (PA : aprop2) : aprop2 :=
+  fun sq sb =>
+    exists sp sa, PA sp sa /\ cds m1 m2 c1 c2 (sp, sa) (sq, sb).
+
+Definition al_underc_r (m1 m2 : mode) (PA : aprop2)
+                       (c1 c2 : astmt) (QB : aprop2) : Prop :=
+  forall sq sb, QB sq sb -> al_postc_r m1 m2 c1 c2 PA sq sb.
+
+Definition aprop2_impl (P Q : aprop2) : Prop := forall sp sa, P sp sa -> Q sp sa.
+Notation "P ==>> Q" := (aprop2_impl P Q) (at level 80).
+
+Reserved Notation
+  "'AL' m1 ',' m2 :: PA |- c1 '//' c2 ==> QB"
+  (at level 90, c1 custom al_stmt at level 99, c2 custom al_stmt at level 99,
+   m1 constr at level 0, m2 constr at level 0,
+   PA constr at level 0, QB constr at level 0).
+
+(** Composed hoare-style proof system *)
+Inductive derivable2 :
+  mode -> mode -> aprop2 -> astmt -> astmt -> aprop2 -> Prop :=
+| D2Par : forall m1 m2 P A c1 c2 Q B,
+    P, [c1] m1, Q ->
+    A, [c2] m2, B ->
+    AL m1 , m2 :: (aprod P A) |- c1 // c2 ==> (aprod Q B)
+| D2Dup : forall P c Q,
+    P, [c] Ok, Q ->
+    AL Ok , Ok :: (aprod P P) |- c // c ==> (aprod Q Q)
+| D2Consequence : forall m1 m2 PA PA' c1 c2 QB QB',
+    PA ==>> PA' ->
+    QB' ==>> QB ->
+    AL m1 , m2 :: PA |- c1 // c2 ==> QB ->
+    AL m1 , m2 :: PA' |- c1 // c2 ==> QB'
+| D2Com : forall m1 m2 (PA : aprop2) c1 c2 (s : id),
+    AL m1 , m2 :: PA |- c1 // c2 ==>
+      (fun sq sb => exists v l1 l2,
+         PA (sq[[ s :=vch v :: l1 ]]) (sb[[ s :=ach l2 ]])
+         /\ sq.(vstate).(ch) s = l1
+         /\ sb.(astate).(ch) s = (l2 ++ [v])%list)
+| D2ComAP : forall m1 m2 (PA : aprop2) c1 c2 (s : id),
+    AL m1 , m2 :: PA |- c1 // c2 ==>
+      (fun sq sb => exists v l1 l2,
+         PA (sq[[ s :=vch l2 ]]) (sb[[ s :=ach v :: l1 ]])
+         /\ sb.(astate).(ch) s = l1
+         /\ sq.(vstate).(ch) s = (l2 ++ [v])%list)
+| D2AdvCons : forall m1 m2 PA c1 c2 (QB extra : aprop2),
+    AL m1 , m2 :: PA |- c1 // c2 ==> QB ->
+    AL m1 , m2 :: PA |- c1 // c2 ==> (fun sq sb => QB sq sb /\ extra sq sb)
+| D2StepL : forall m1 m2 P c1 Q (K : aprop),
+    P, [c1] m1, Q ->
+    AL m1 , m2 :: (fun sp sa => P sp /\ K sa) |- c1 // skip
+              ==> (fun sq sb => Q sq /\ K sb)
+| D2StepR : forall m1 m2 (K : aprop) A c2 B,
+    A, [c2] m2, B ->
+    AL m1 , m2 :: (fun sp sa => K sp /\ A sa) |- skip // c2
+              ==> (fun sq sb => K sq /\ B sb)
+where "'AL' m1 ',' m2 :: PA |- c1 '//' c2 ==> QB" :=
+  (derivable2 m1 m2 PA c1 c2 QB).
+
+Lemma vch_shadow : forall sig s l l',
+  sig[[ s :=vch l ]] [[ s :=vch l' ]] = sig[[ s :=vch l' ]].
+Proof.
+  intros ((vs & vc) & (as_ & ac)) s l l'. unfold update_vchannel. simpl.
+  now rewrite update_shadow.
+Qed.
+
+Lemma ach_shadow : forall sig s l l',
+  sig[[ s :=ach l ]] [[ s :=ach l' ]] = sig[[ s :=ach l' ]].
+Proof.
+  intros ((vs & vc) & (as_ & ac)) s l l'. unfold update_achannel. simpl.
+  now rewrite update_shadow.
+Qed.
+
+Lemma vch_eq : forall sig s l,
+  sig.(vstate).(ch) s = l -> sig[[ s :=vch l ]] = sig.
+Proof.
+  intros ((vs & vc) & (as_ & ac)) s l H. unfold update_vchannel. simpl in *.
+  now rewrite (state_upd_eq _ vc s l H).
+Qed.
+
+Lemma ach_eq : forall sig s l,
+  sig.(astate).(ch) s = l -> sig[[ s :=ach l ]] = sig.
+Proof.
+  intros ((vs & vc) & (as_ & ac)) s l H. unfold update_achannel. simpl in *.
+  now rewrite (state_upd_eq _ ac s l H).
+Qed.
+
+Lemma vch_get : forall sig s l, (sig[[ s :=vch l ]]).(vstate).(ch) s = l.
+Proof.
+  intros ((vs & vc) & (as_ & ac)) s l. unfold update_vchannel. simpl. now rewrite update_eq.
+Qed.
+Lemma ach_get : forall sig s l, (sig[[ s :=ach l ]]).(astate).(ch) s = l.
+Proof.
+  intros ((vs & vc) & (as_ & ac)) s l. unfold update_achannel. simpl. now rewrite update_eq.
+Qed.
+
+Lemma vch_neq : forall sig j k l,
+  j <> k -> (sig[[ j :=vch l ]]).(vstate).(ch) k = sig.(vstate).(ch) k.
+Proof.
+  intros ((vs & vc) & (as_ & ac)) j k l Hneq. unfold update_vchannel. simpl.
+  now apply update_neq.
+Qed.
+Lemma ach_neq : forall sig j k l,
+  j <> k -> (sig[[ j :=ach l ]]).(astate).(ch) k = sig.(astate).(ch) k.
+Proof.
+  intros ((vs & vc) & (as_ & ac)) j k l Hneq. unfold update_achannel. simpl.
+  now apply update_neq.
+Qed.
+
+Lemma vch_vstore_upd : forall sig x v k,
+  (sig[[ x :=v v ]]).(vstate).(ch) k = sig.(vstate).(ch) k.
+Proof. intros. reflexivity. Qed.
+Lemma ach_vstore_upd : forall sig x v k,
+  (sig[[ x :=v v ]]).(astate).(ch) k = sig.(astate).(ch) k.
+Proof. intros. reflexivity. Qed.
+Lemma vch_astore_upd : forall sig x v k,
+  (sig[[ x :=a v ]]).(vstate).(ch) k = sig.(vstate).(ch) k.
+Proof. intros. reflexivity. Qed.
+Lemma ach_astore_upd : forall sig x v k,
+  (sig[[ x :=a v ]]).(astate).(ch) k = sig.(astate).(ch) k.
+Proof. intros. reflexivity. Qed.
+Lemma ach_vchan_upd : forall sig j l k,
+  (sig[[ j :=vch l ]]).(astate).(ch) k = sig.(astate).(ch) k.
+Proof. intros. reflexivity. Qed.
+Lemma vch_achan_upd : forall sig j l k,
+  (sig[[ j :=ach l ]]).(vstate).(ch) k = sig.(vstate).(ch) k.
+Proof. intros. reflexivity. Qed.
+(* store read is unaffected by channel updates on the same side *)
+Lemma astore_achan_upd : forall sig j l k,
+  (sig[[ j :=ach l ]]).(astate).(s) k = sig.(astate).(s) k.
+Proof. intros. reflexivity. Qed.
+Lemma vstore_vchan_upd : forall sig j l k,
+  (sig[[ j :=vch l ]]).(vstate).(s) k = sig.(vstate).(s) k.
+Proof. intros. reflexivity. Qed.
+
+Lemma mode_chan_upd_Ok : forall sig k l, mode_chan_upd Ok sig k l = sig[[ k :=vch l ]].
+Proof. reflexivity. Qed.
+Lemma mode_chan_upd_Ad : forall sig k l, mode_chan_upd Ad sig k l = sig[[ k :=ach l ]].
+Proof. reflexivity. Qed.
+Lemma mode_upd_Ok : forall sig x v, mode_upd Ok sig x v = sig[[ x :=v v ]].
+Proof. reflexivity. Qed.
+Lemma mode_upd_Ad : forall sig x v, mode_upd Ad sig x v = sig[[ x :=a v ]].
+Proof. reflexivity. Qed.
+Lemma mode_chan_Ok : forall sig k, mode_chan Ok sig k = sig.(vstate).(ch) k.
+Proof. reflexivity. Qed.
+Lemma mode_chan_Ad : forall sig k, mode_chan Ad sig k = sig.(astate).(ch) k.
+Proof. reflexivity. Qed.
+Lemma mode_store_Ok : forall sig, mode_store Ok sig = sig.(vstate).(s).
+Proof. reflexivity. Qed.
+Lemma mode_store_Ad : forall sig, mode_store Ad sig = sig.(astate).(s).
+Proof. reflexivity. Qed.
+Lemma astore_aupd_eq : forall sig x v, (sig[[ x :=a v ]]).(astate).(s) x = v.
+Proof. intros. apply update_eq. Qed.
+Lemma vstore_vupd_eq : forall sig x v, (sig[[ x :=v v ]]).(vstate).(s) x = v.
+Proof. intros. apply update_eq. Qed.
+
+(* Raw-notation "different key"/"other record" store-read independence
+   lemmas, completing the cross-product ({vstate,astate}.s reads against
+   {[[:=v]],[[:=a]],[[:=vch]],[[:=ach]]} raw updates) that [vch_neq]/[ach_neq]
+   and [vstore_vchan_upd]/[astore_achan_upd] leave uncovered.  Needed once a
+   store read has to be traced back through a MIX of raw-notation updates
+   (as produced by chaining [D2Com]/[D2ComAP] postconditions without a [set]
+   to name each intermediate state) rather than the [mode_upd]/[mode_chan_upd]
+   function forms the [astore_mode_upd_Ok]-family already covers. *)
+Lemma vstore_vupd_neq : forall sig x y v,
+  y <> x -> (sig[[ y :=v v ]]).(vstate).(s) x = sig.(vstate).(s) x.
+Proof.
+  intros ((vs & vc) & (as_ & ac)) x y v Hneq. unfold update_victim. simpl.
+  now apply update_neq.
+Qed.
+Lemma astore_aupd_neq : forall sig x y v,
+  y <> x -> (sig[[ y :=a v ]]).(astate).(s) x = sig.(astate).(s) x.
+Proof.
+  intros ((vs & vc) & (as_ & ac)) x y v Hneq. unfold update_adversary. simpl.
+  now apply update_neq.
+Qed.
+Lemma vstore_aupd_upd : forall sig x y v,
+  (sig[[ y :=a v ]]).(vstate).(s) x = sig.(vstate).(s) x.
+Proof. intros. reflexivity. Qed.
+Lemma astore_vupd_upd : forall sig x y v,
+  (sig[[ y :=v v ]]).(astate).(s) x = sig.(astate).(s) x.
+Proof. intros. reflexivity. Qed.
+Lemma vstore_achan_upd : forall sig j l x,
+  (sig[[ j :=ach l ]]).(vstate).(s) x = sig.(vstate).(s) x.
+Proof. intros. reflexivity. Qed.
+Lemma astore_vchan_upd : forall sig j l x,
+  (sig[[ j :=vch l ]]).(astate).(s) x = sig.(astate).(s) x.
+Proof. intros. reflexivity. Qed.
+
+Lemma mode_chan_mode_upd : forall m sig x v k,
+  mode_chan m (mode_upd m sig x v) k = mode_chan m sig k.
+Proof. intros. destruct m; [apply vch_vstore_upd | apply ach_astore_upd]. Qed.
+
+Lemma mode_store_mode_chan_upd : forall m sig k l x,
+  mode_store m (mode_chan_upd m sig k l) x = mode_store m sig x.
+Proof. intros. destruct m; [apply vstore_vchan_upd | apply astore_achan_upd]. Qed.
+
+Lemma mode_store_mode_upd_neq : forall m sig y v x,
+  y <> x -> mode_store m (mode_upd m sig y v) x = mode_store m sig x.
+Proof. intros m sig y v x Hneq. destruct m; simpl; now apply update_neq. Qed.
+
+Lemma mode_chan_get : forall m sig k l,
+  mode_chan m (mode_chan_upd m sig k l) k = l.
+Proof. intros. destruct m; [apply vch_get | apply ach_get]. Qed.
+
+Lemma mode_chan_upd_shadow : forall m sig k l l',
+  mode_chan_upd m (mode_chan_upd m sig k l) k l' = mode_chan_upd m sig k l'.
+Proof. intros. destruct m; [apply vch_shadow | apply ach_shadow]. Qed.
+
+Lemma mode_chan_upd_eq : forall m sig k,
+  mode_chan_upd m sig k (mode_chan m sig k) = sig.
+Proof. intros. destruct m; [apply vch_eq | apply ach_eq]; reflexivity. Qed.
+
+(** Lemmas to concretize the application of DRS rules *)
+Section ConcreteStepHelpers.
+
+Lemma DAssign_concrete : forall m x (e : expression) X,
+  (fun sig => sig = X), [x := e] m,
+    (fun sig => sig = mode_upd m X x (e (mode_store m X))).
+Proof.
+  intros m x e X. eapply DConsequence with (P := fun sig => sig = X).
+  3: apply DAssign.
+  - intros sig ->. reflexivity.
+  - intros sig ->.
+    exists (mode_store m X x).
+    rewrite mode_upd_shadow, mode_upd_store_eq.
+    split. reflexivity.
+    now rewrite mode_store_upd_eq.
+Qed.
+
+Lemma DRead_concrete : forall m (chn x : id) X v l,
+  mode_chan m X chn = v :: l ->
+  (fun sig => sig = X), [read(chn, x)] m,
+    (fun sig => sig = mode_chan_upd m (mode_upd m X x v) chn l).
+Proof.
+  intros m chn x X v l Hchan. eapply DConsequence with (P := fun sig => sig = X).
+  3: apply DRead.
+  - intros sig ->. reflexivity.
+  - intros sig ->.
+    exists v, (mode_store m X x), l.
+    assert (Hundo :
+      mode_chan_upd m (mode_upd m (mode_chan_upd m (mode_upd m X x v) chn l)
+                          x (mode_store m X x)) chn (v :: l) = X).
+    { revert Hchan. destruct m; destruct X as [(vs & vc) (as_ & ac)]; intros Hchan;
+        simpl in *;
+        unfold update_vchannel, update_victim,
+               update_achannel, update_adversary in *; simpl in *;
+        f_equal; f_equal;
+        first [ reflexivity
+              | now rewrite update_shadow, state_upd_eq
+              | now rewrite update_shadow, <- Hchan, state_upd_eq ]. }
+    repeat split.
+    + exact Hundo.
+    + rewrite mode_chan_get. reflexivity.
+    + rewrite mode_store_mode_chan_upd. now rewrite mode_store_upd_eq.
+Qed.
+
+Lemma DWrite_concrete : forall m (chn x : id) X,
+  (fun sig => sig = X), [write(chn, x)] m,
+    (fun sig => sig = mode_chan_upd m X chn
+                  (mode_chan m X chn ++ [mode_store m X x])%list).
+Proof.
+  intros m chn x X. eapply DConsequence with (P := fun sig => sig = X).
+  3: apply DWrite.
+  - intros sig ->. reflexivity.
+  - intros sig ->.
+    exists (mode_chan m X chn). split.
+    + rewrite mode_chan_upd_shadow. apply mode_chan_upd_eq.
+    + rewrite mode_chan_get, mode_store_mode_chan_upd. reflexivity.
+Qed.
+
+Lemma DAssume_concrete : forall m (B : prop) X,
+  B (mode_store m X) ->
+  (fun sig => sig = X), [assume(B)] m, (fun sig => sig = X).
+Proof.
+  intros m B X HB. eapply DConsequence with (P := fun sig => sig = X).
+  3: apply DAssume.
+  - intros sig ->. reflexivity.
+  - intros sig ->. split. reflexivity. exact HB.
+Qed.
+
+Lemma astore_mode_upd_Ok : forall sig y v x,
+  mode_store Ad (mode_upd Ok sig y v) x = mode_store Ad sig x.
+Proof. reflexivity. Qed.
+Lemma astore_mode_chan_upd_Ok : forall sig k l x,
+  mode_store Ad (mode_chan_upd Ok sig k l) x = mode_store Ad sig x.
+Proof. reflexivity. Qed.
+Lemma vstore_mode_upd_Ad : forall sig y v x,
+  mode_store Ok (mode_upd Ad sig y v) x = mode_store Ok sig x.
+Proof. reflexivity. Qed.
+Lemma vstore_mode_chan_upd_Ad : forall sig k l x,
+  mode_store Ok (mode_chan_upd Ad sig k l) x = mode_store Ok sig x.
+Proof. reflexivity. Qed.
+
+End ConcreteStepHelpers.
+
+(** Soundness of the composed system with respect to the composed semantics [al_underc_r]. *)
+Section Tier2Soundness.
+
+Theorem soundness2 :
+  forall m1 m2 PA c1 c2 QB,
+    AL m1 , m2 :: PA |- c1 // c2 ==> QB ->
+    al_underc_r m1 m2 PA c1 c2 QB.
+Proof.
+  intros m1 m2 PA c1 c2 QB H. induction H.
+  - (* D2Par *)
+    apply soundness in H. apply soundness in H0.
+    intros sq sb (Qsq & Bsb).
+    destruct (H sq Qsq) as (sp & Psp & DS1).
+    destruct (H0 sb Bsb) as (sa & Asa & DS2).
+    exists sp, sa. split. split; assumption. now apply CInd.
+  - (* D2Dup *)
+    apply soundness in H.
+    intros sq sb (Qsq & Qsb).
+    destruct (H sq Qsq) as (sp & Psp & DS1).
+    destruct (H sb Qsb) as (sa & Psa & DS2).
+    exists sp, sa. split. split; assumption. now apply CInd.
+  - (* D2Consequence *)
+    intros sq sb QB'sq. apply H0 in QB'sq.
+    destruct (IHderivable2 sq sb QB'sq) as (sp & sa & PAsp & DS).
+    exists sp, sa. split. now apply H. assumption.
+  - (* D2Com *)
+    intros sq sb (v & l1 & l2 & PApre & Hq & Hb).
+    exists (sq[[ s :=vch v :: l1 ]]), (sb[[ s :=ach l2 ]]).
+    split. assumption.
+    replace sq with ((sq[[ s :=vch v :: l1 ]])[[ s :=vch l1 ]]) at 2
+      by (rewrite vch_shadow; now apply vch_eq).
+    replace sb with ((sb[[ s :=ach l2 ]])[[ s :=ach (l2 ++ [v])%list ]]) at 2
+      by (rewrite ach_shadow; apply ach_eq; now rewrite Hb).
+    apply CComPA.
+    + now rewrite vch_get.
+    + now rewrite ach_get.
+  - (* D2ComAP *)
+    intros sq sb (v & l1 & l2 & PApre & Hb & Hq).
+    exists (sq[[ s :=vch l2 ]]), (sb[[ s :=ach v :: l1 ]]).
+    split. assumption.
+    replace sq with ((sq[[ s :=vch l2 ]])[[ s :=vch (l2 ++ [v])%list ]]) at 2
+      by (rewrite vch_shadow; apply vch_eq; now rewrite Hq).
+    replace sb with ((sb[[ s :=ach v :: l1 ]])[[ s :=ach l1 ]]) at 2
+      by (rewrite ach_shadow; now apply ach_eq).
+    apply CComAP.
+    + now rewrite ach_get.
+    + now rewrite vch_get.
+  - (* D2AdvCons *)
+    intros sq sb (QBsq & extrasq).
+    destruct (IHderivable2 sq sb QBsq) as (sp & sa & PAsp & DS).
+    exists sp, sa. split; assumption.
+  - (* D2StepL *)
+    apply soundness in H.
+    intros sq sb (Qsq & Ksb).
+    destruct (H sq Qsq) as (sp & Psp & DS1).
+    exists sp, sb. split. split; assumption.
+    apply CInd. exact DS1. apply EDSkip.
+  - (* D2StepR *)
+    apply soundness in H.
+    intros sq sb (Ksq & Bsb).
+    destruct (H sb Bsb) as (sa & Asa & DS2).
+    exists sq, sa. split. split; assumption.
+    apply CInd. apply EDSkip. exact DS2.
+Qed.
+
+Lemma derivable2_cds_step : forall m1 m2 c1 c2 X Y X' Y' QB,
+  QB X' Y' ->
+  AL m1 , m2 :: (fun sp sa => sp = X /\ sa = Y) |- c1 // c2 ==> QB ->
+  cds m1 m2 c1 c2 (X, Y) (X', Y').
+Proof.
+  intros m1 m2 c1 c2 X Y X' Y' QB HQB Hderiv.
+  apply soundness2 in Hderiv.
+  destruct (Hderiv X' Y' HQB) as (sp & sa & (-> & ->) & Hcds).
+  exact Hcds.
+Qed.
+
+End Tier2Soundness.
+
+(** Adversarial Consequence *)
+
+Section AdversarialConsequence.
+
+Definition closed_aprop (Q : aprop) : Prop :=
+  forall sig sig', Q sig <-> Q sig'.
+
+(* The closed program fact [Q] holds and the adversary-side variable [v2] equals
+   some witnessed [v1]. *)
+Definition advcons_payload (Q : aprop) (v2 : id) : aprop2 :=
+  fun _sq sb => exists v1, Q sb /\ mode_store Ad sb v2 = v1.
+
+(* Derived Adversarial Consequence *)
+Theorem D2AdvCons_payload :
+  forall m1 m2 PA c1 c2 QB (Q : aprop) (v2 : id),
+    closed_aprop Q ->
+    AL m1 , m2 :: PA |- c1 // c2 ==> QB ->
+    AL m1 , m2 :: PA |- c1 // c2 ==>
+      (fun sq sb => QB sq sb /\ advcons_payload Q v2 sq sb).
+Proof.
+  intros m1 m2 PA c1 c2 QB Q v2 _Hclosed Hd.
+  apply (D2AdvCons m1 m2 PA c1 c2 QB (advcons_payload Q v2)). exact Hd.
+Qed.
+
+End AdversarialConsequence.
+
+(** Parallel Backward Variant *)
+Section PBV.
+
+Lemma cds_star_trans : forall m1 m2 c1 c2 p q r,
+  cds_star m1 m2 c1 c2 p q ->
+  cds_star m1 m2 c1 c2 q r ->
+  cds_star m1 m2 c1 c2 p r.
+Proof.
+  intros m1 m2 c1 c2 p q r Hpq Hqr. induction Hqr.
+  - assumption.
+  - eapply CSN; [ apply IHHqr; assumption | assumption ].
+Qed.
+
+Lemma cds_cds_star : forall m1 m2 c1 c2 p q,
+  cds m1 m2 c1 c2 p q -> cds_star m1 m2 c1 c2 p q.
+Proof. intros. eapply CSN. apply CS0. assumption. Qed.
+
+Lemma cds_star_hetero_trans : forall m1 m2 p q r,
+  cds_star_hetero m1 m2 p q ->
+  cds_star_hetero m1 m2 q r ->
+  cds_star_hetero m1 m2 p r.
+Proof.
+  intros m1 m2 p q r Hpq Hqr. revert p Hpq. induction Hqr; intros p1 Hp1.
+  - assumption.
+  - eapply CSHN. apply IHHqr. exact Hp1. exact H.
+Qed.
+
+Lemma cds_cds_star_hetero : forall m1 m2 c1 c2 p q,
+  cds m1 m2 c1 c2 p q -> cds_star_hetero m1 m2 p q.
+Proof. intros m1 m2 c1 c2 p q H. eapply CSHN. apply CSH0. exact H. Qed.
+
+Definition PBV_premise (m1 m2 : mode) (P A : nat -> aprop) (c1 c2 : astmt)
+           (pred : nat -> nat -> (nat * nat)) : Prop :=
+  forall n' m', (n' + m' > 0)%nat ->
+    let (n, m) := pred n' m' in
+    (n + m < n' + m')%nat /\
+    al_underc_r m1 m2 (aprod (P n) (A m)) c1 c2 (aprod (P n') (A m')).
+
+(* Every [(P n', A m')] post-pair is reachable by [cds_star] from a [(P 0, A 0)] pre-pair. *)
+Lemma PBV_reach :
+  forall m1 m2 (P A : nat -> aprop) c1 c2 pred,
+    PBV_premise m1 m2 P A c1 c2 pred ->
+    forall k n' m', (n' + m' <= k)%nat ->
+      forall sq sb, P n' sq -> A m' sb ->
+        exists sp sa, P 0%nat sp /\ A 0%nat sa /\
+                      cds_star m1 m2 c1 c2 (sp, sa) (sq, sb).
+Proof.
+  intros m1 m2 P A c1 c2 pred Hprem k.
+  induction k as [ | k IH ]; intros n' m' Hle sq sb HP HA.
+  - assert (n' = 0 /\ m' = 0)%nat as [-> ->] by (split; lia).
+    exists sq, sb. repeat split; try assumption. apply CS0.
+  - (* k = S k *)
+    destruct (Nat.eq_dec (n' + m')%nat 0) as [E0 | Epos].
+    + assert (n' = 0 /\ m' = 0)%nat as [-> ->] by (split; lia).
+      exists sq, sb. repeat split; try assumption. apply CS0.
+    + assert (Hpos : (n' + m' > 0)%nat) by lia.
+      specialize (Hprem n' m' Hpos).
+      destruct (pred n' m') as (n, m).
+      destruct Hprem as (Hlt & Htriple).
+      destruct (Htriple sq sb (conj HP HA)) as (sp & sa & (Psp & Asa) & DS).
+      assert (Hsmaller : (n + m <= k)%nat) by lia.
+      destruct (IH n m Hsmaller sp sa Psp Asa)
+        as (sp0 & sa0 & P0 & A0 & Star0).
+      exists sp0, sa0. repeat split; try assumption.
+      eapply cds_star_trans. apply Star0. now apply cds_cds_star.
+Qed.
+
+Theorem PBV_sound :
+  forall m1 m2 (P A : nat -> aprop) c1 c2 pred,
+    PBV_premise m1 m2 P A c1 c2 pred ->
+    al_underc_star m1 m2 (aprod (P 0%nat) (A 0%nat)) c1 c2
+      (fun sq sb => (exists n, P n sq) /\ (exists m, A m sb)).
+Proof.
+  intros m1 m2 P A c1 c2 pred Hprem sq sb ((n' & HP) & (m' & HA)).
+  destruct (PBV_reach m1 m2 P A c1 c2 pred Hprem (n' + m')%nat n' m'
+              (le_n _) sq sb HP HA)
+    as (sp & sa & P0 & A0 & Star).
+  exists sp, sa. split; [ split; assumption | assumption ].
+Qed.
+
+End PBV.
+
+(** PBV over a multi-step round *)
+Section PBVMultiStep.
+
+Definition PBV_premise_star (m1 m2 : mode) (P A : nat -> aprop) (c1 c2 : astmt)
+           (pred : nat -> nat -> (nat * nat)) : Prop :=
+  forall n' m', (n' + m' > 0)%nat ->
+    let (n, m) := pred n' m' in
+    (n + m < n' + m')%nat /\
+    al_underc_star m1 m2 (aprod (P n) (A m)) c1 c2 (aprod (P n') (A m')).
+
+Lemma PBV_reach_star :
+  forall m1 m2 (P A : nat -> aprop) c1 c2 pred,
+    PBV_premise_star m1 m2 P A c1 c2 pred ->
+    forall k n' m', (n' + m' <= k)%nat ->
+      forall sq sb, P n' sq -> A m' sb ->
+        exists sp sa, P 0%nat sp /\ A 0%nat sa /\
+                      cds_star m1 m2 c1 c2 (sp, sa) (sq, sb).
+Proof.
+  intros m1 m2 P A c1 c2 pred Hprem k.
+  induction k as [ | k IH ]; intros n' m' Hle sq sb HP HA.
+  - assert (n' = 0 /\ m' = 0)%nat as [-> ->] by (split; lia).
+    exists sq, sb. repeat split; try assumption. apply CS0.
+  - destruct (Nat.eq_dec (n' + m')%nat 0) as [E0 | Epos].
+    + assert (n' = 0 /\ m' = 0)%nat as [-> ->] by (split; lia).
+      exists sq, sb. repeat split; try assumption. apply CS0.
+    + assert (Hpos : (n' + m' > 0)%nat) by lia.
+      specialize (Hprem n' m' Hpos).
+      destruct (pred n' m') as (n, m).
+      destruct Hprem as (Hlt & Htriple).
+      destruct (Htriple sq sb (conj HP HA)) as (sp & sa & (Psp & Asa) & Star).
+      assert (Hsmaller : (n + m <= k)%nat) by lia.
+      destruct (IH n m Hsmaller sp sa Psp Asa)
+        as (sp0 & sa0 & P0 & A0 & Star0).
+      exists sp0, sa0. repeat split; try assumption.
+      eapply cds_star_trans. apply Star0. exact Star.
+Qed.
+
+Theorem PBV_sound_star :
+  forall m1 m2 (P A : nat -> aprop) c1 c2 pred,
+    PBV_premise_star m1 m2 P A c1 c2 pred ->
+    al_underc_star m1 m2 (aprod (P 0%nat) (A 0%nat)) c1 c2
+      (fun sq sb => (exists n, P n sq) /\ (exists m, A m sb)).
+Proof.
+  intros m1 m2 P A c1 c2 pred Hprem sq sb ((n' & HP) & (m' & HA)).
+  destruct (PBV_reach_star m1 m2 P A c1 c2 pred Hprem (n' + m')%nat n' m'
+              (le_n _) sq sb HP HA)
+    as (sp & sa & P0 & A0 & Star).
+  exists sp, sa. split; [ split; assumption | assumption ].
+Qed.
+
+End PBVMultiStep.
+
+(* Frame rule / constancy *)
+Section Framing.
+
+(* Variables a command may write to *)
+Fixpoint Mod (c : astmt) : list id :=
+  match c with
+  | ASkip => nil
+  | AAssign x _ => x :: nil
+  | ARand x => x :: nil
+  | ASeq c1 c2 => Mod c1 ++ Mod c2
+  | APar c1 c2 => Mod c1 ++ Mod c2
+  | AAssume _ => nil
+  | AStar c => Mod c
+  | AChoice c1 c2 => Mod c1 ++ Mod c2
+  | ARead _ x => x :: nil
+  | AWrite _ _ => nil
+  | AAdvAssert _ => nil
+  | ACom c1 c2 => nil
+  | ALocal _ _ c => Mod c
+  end.
+
+(* Channels a command may write to *)
+Fixpoint ModCh (c : astmt) : list id :=
+  match c with
+  | ASkip => nil
+  | AAssign _ _ => nil
+  | ARand _ => nil
+  | ASeq c1 c2 => ModCh c1 ++ ModCh c2
+  | APar c1 c2 => ModCh c1 ++ ModCh c2
+  | AAssume _ => nil
+  | AStar c => ModCh c
+  | AChoice c1 c2 => ModCh c1 ++ ModCh c2
+  | ARead s _ => s :: nil
+  | AWrite s _ => s :: nil
+  | AAdvAssert _ => nil
+  | ACom c1 c2 => nil
+  | ALocal _ _ c => ModCh c
+  end.
+
+(* [F] does not depend, in mode [m]'s store, on any variable in [V] or any channel in [C]. *)
+Definition indep (m : mode) (V C : list id) (F : aprop) : Prop :=
+  (forall sig x v, In x V -> (F (mode_upd m sig x v) <-> F sig))
+  /\ (forall sig k l, In k C -> (F (mode_chan_upd m sig k l) <-> F sig)).
+
+Lemma in_app_l : forall (x:id) l1 l2, In x l1 -> In x (l1 ++ l2).
+Proof. intros. apply in_or_app. now left. Qed.
+Lemma in_app_r : forall (x:id) l1 l2, In x l2 -> In x (l1 ++ l2).
+Proof. intros. apply in_or_app. now right. Qed.
+
+Lemma indep_sub : forall m V V' C C' F,
+  (forall x, In x V -> In x V') ->
+  (forall k, In k C -> In k C') ->
+  indep m V' C' F -> indep m V C F.
+Proof.
+  intros m V V' C C' F HV HC [Hv Hc]. split; intros.
+  - apply Hv. now apply HV.
+  - apply Hc. now apply HC.
+Qed.
+
+(* NOTE : give a very simple explanation for this *)
+Fixpoint ComFree (c : astmt) : Prop :=
+  match c with
+  | ASkip | AAssign _ _ | ARand _ | AAssume _ | ARead _ _ | AWrite _ _
+  | AAdvAssert _ => True
+  | ASeq c1 c2 | APar c1 c2 | AChoice c1 c2 => ComFree c1 /\ ComFree c2
+  | AStar c => ComFree c
+  | ALocal _ _ c => False
+  | ACom _ _ => False
+  end.
+
+(* A [ds] step of a [Com]-free command changes only [Mod c] variables and
+   [ModCh c] channels of the active store *)
+Lemma frame_ds : forall c m sig sig',
+  ds c m (sig, sig') ->
+  ComFree c ->
+  forall F, indep m (Mod c) (ModCh c) F -> (F sig <-> F sig').
+Proof.
+  intros c m sig sig' H.
+  remember (sig, sig') as pr eqn:E.
+  revert sig sig' E.
+  induction H; intros sig0 sig0' E CF F Hindep;
+    inversion E; subst; clear E; try tauto.
+  - inversion Hindep; subst; clear Hindep.
+    rewrite H. reflexivity. simpl. now left.
+  - destruct Hindep as [Hv _]. simpl in Hv.
+    specialize (Hv sig0 x (e (sig0.(astate).(s))) (or_introl eq_refl)).
+    simpl in Hv. symmetry. exact Hv.
+  - destruct Hindep as [Hv _]. simpl in Hv.
+    specialize (Hv sig0 x v (or_introl eq_refl)). simpl in Hv. symmetry. exact Hv.
+  - destruct Hindep as [Hv _]. simpl in Hv.
+    specialize (Hv sig0 x v (or_introl eq_refl)). simpl in Hv. symmetry. exact Hv.
+  - destruct CF as [CF1 CF2].
+    assert (I1 : indep m (Mod c1) (ModCh c1) F).
+    { apply (indep_sub m (Mod c1) (Mod c1 ++ Mod c2)
+                         (ModCh c1) (ModCh c1 ++ ModCh c2));
+        [ intros; now apply in_app_l | intros; now apply in_app_l | exact Hindep ]. }
+    assert (I2 : indep m (Mod c2) (ModCh c2) F).
+    { apply (indep_sub m (Mod c2) (Mod c1 ++ Mod c2)
+                         (ModCh c2) (ModCh c1 ++ ModCh c2));
+        [ intros; now apply in_app_r | intros; now apply in_app_r | exact Hindep ]. }
+    rewrite (IHds1 _ _ eq_refl CF1 F I1).
+    now apply (IHds2 _ _ eq_refl CF2 F I2).
+  - destruct Hindep as [Hv Hc]. simpl in Hv, Hc.
+    specialize (Hv sig0 x v (or_introl eq_refl)). simpl in Hv.
+    specialize (Hc (sig0[[ x :=v v ]]) s l (or_introl eq_refl)). simpl in Hc.
+    now rewrite Hc, Hv.
+  - destruct Hindep as [Hv Hc]. simpl in Hv, Hc.
+    rewrite Hc, Hv; intuition.
+  - destruct Hindep as [_ Hc]. simpl in Hc.
+    rewrite Hc; intuition.
+  - destruct Hindep as [_ Hc]. simpl in Hc.
+    rewrite Hc; intuition.
+  - apply IHds; eauto.
+      apply CF.
+    eapply indep_sub; [| |eassumption];
+      intros; now apply in_app_l.
+  - apply IHds; eauto.
+      apply CF.
+    eapply indep_sub; [| |eassumption];
+      intros; now apply in_app_r.
+  - rewrite IHds1. apply IHds2. all: intuition.
+  - destruct CF as [CF1 CF2].
+    apply IHds; intuition.
+    eapply indep_sub; [| |eassumption];
+      intros; simpl; now apply in_app_l.
+  - destruct CF as [CF1 CF2].
+    apply IHds; intuition.
+    eapply indep_sub; [| |eassumption];
+      intros; simpl; now apply in_app_r.
+  - destruct CF.
+  - destruct CF.
+  - destruct CF.
+Qed.
+
+Theorem constancy :
+  forall P Q c m F,
+    ComFree c ->
+    indep m (Mod c) (ModCh c) F ->
+    {{ P }} c [[m]] {{ Q }} ->
+    {{ aand P F }} c [[m]] {{ aand Q F }}.
+Proof.
+  intros P Q c m F CF Hindep HU sig (Qsig & Fsig).
+  destruct (HU sig Qsig) as (sig0 & Psig0 & DS).
+  exists sig0. split.
+  - split. assumption.
+    apply (frame_ds c m sig0 sig DS CF F Hindep). exact Fsig.
+  - assumption.
+Qed.
+
+End Framing.
+
+(** Small-step interleaving semantics to represent paper examples
+
+    [sstep m c sig c' sig'] : in mode [m], command [c] in state [sig] takes one
+    step to [c'] and [sig']. *)
+
+Section SmallStepSemantics.
+
+Inductive sstep : mode -> astmt -> estate -> astmt -> estate -> Prop :=
+| SAssign : forall m x e sig,
+    sstep m (AAssign x e) sig ASkip (mode_upd m sig x (e (mode_store m sig)))
+| SRand : forall m x v sig,
+    sstep m (ARand x) sig ASkip (mode_upd m sig x v)
+| SAssume : forall m (B : prop) sig,
+    B (mode_store m sig) ->
+    sstep m (AAssume B) sig ASkip sig
+| SRead : forall m s x v l sig,
+    mode_chan m sig s = v :: l ->
+    sstep m (ARead s x) sig ASkip (mode_chan_upd m (mode_upd m sig x v) s l)
+| SWrite : forall m s x sig,
+    sstep m (AWrite s x) sig ASkip
+          (mode_chan_upd m sig s (mode_chan m sig s ++ [mode_store m sig x])%list)
+| SAdvAssertS : forall (P : prop) sig,
+    P (sig.(astate).(s)) ->
+    sstep Ad (AAdvAssert P) sig ASkip sig
+| SAdvAssertF : forall (P : prop) sig,
+    ~ P (sig.(astate).(s)) ->
+    sstep Ad (AAdvAssert P) sig ASkip sig
+| SSeqSkip : forall m c2 sig,
+    sstep m (ASeq ASkip c2) sig c2 sig
+| SSeqStep : forall m c1 c1' c2 sig sig',
+    sstep m c1 sig c1' sig' ->
+    sstep m (ASeq c1 c2) sig (ASeq c1' c2) sig'
+| SChoiceL : forall m c1 c2 sig, sstep m (AChoice c1 c2) sig c1 sig
+| SChoiceR : forall m c1 c2 sig, sstep m (AChoice c1 c2) sig c2 sig
+| SStar0 : forall m c sig, sstep m (AStar c) sig ASkip sig
+| SStarN : forall m c sig, sstep m (AStar c) sig (ASeq c (AStar c)) sig
+| SLocalEnter : forall m x e c sig,
+    sstep m (ALocal x e c) sig
+          (ASeq (AAssign x e)
+                (ASeq c (AAssign x (fun _ => mode_store m sig x)))) sig.
+
+Inductive sstep_star (m : mode) : astmt -> estate -> astmt -> estate -> Prop :=
+| SS0 : forall c sig, sstep_star m c sig c sig
+| SSN : forall c sig c' sig' c'' sig'',
+    sstep m c sig c' sig' ->
+    sstep_star m c' sig' c'' sig'' ->
+    sstep_star m c sig c'' sig''.
+
+Lemma sstep_star_trans : forall m c1 s1 c2 s2 c3 s3,
+  sstep_star m c1 s1 c2 s2 -> sstep_star m c2 s2 c3 s3 ->
+  sstep_star m c1 s1 c3 s3.
+Proof.
+  intros m c1 s1 c2 s2 c3 s3 H1 H2. induction H1.
+  - exact H2.
+  - eapply SSN. exact H. apply IHsstep_star. exact H2.
+Qed.
+
+(** Small-step runs are valid big-step executions *)
+Section Adequacy.
+
+Lemma ds_star_left : forall c m a b d,
+  ds c m (a, b) -> ds (AStar c) m (b, d) -> ds (AStar c) m (a, d).
+Proof.
+  intros c m a b d Hc Hstar.
+  remember (AStar c) as sc eqn:E. remember (b, d) as bd eqn:Ebd.
+  revert c a b d Hc E Ebd. induction Hstar; intros c0 a0 b0 d0 Hc E Ebd;
+    try discriminate E.
+  - injection E as ->. injection Ebd as -> ->.
+    eapply EDStarN. apply EDStar0. exact Hc.
+  - injection E as ->. injection Ebd as <- <-.
+    eapply EDStarN.
+    + eapply IHHstar1. exact Hc. reflexivity. reflexivity.
+    + exact Hstar2.
+Qed.
+
+Lemma ds_local_desugar : forall m x e c sig sig'',
+  ds (ASeq (AAssign x e)
+           (ASeq c (AAssign x (fun _ => mode_store m sig x)))) m (sig, sig'') ->
+  ds (ALocal x e c) m (sig, sig'').
+Proof.
+  intros m x e c sig sig'' H.
+  inversion H; subst; clear H.
+  inversion H6; subst; clear H6.
+  destruct m; simpl in *.
+  - inversion H4; subst; clear H4. inversion H7; subst; clear H7.
+    eauto using EDLocal.
+  - inversion H4; subst. inversion H7; subst.
+    eauto using EDLocal.
+Qed.
+
+Lemma sstep_expansion : forall m c sig c' sig',
+  sstep m c sig c' sig' ->
+  forall sig'', ds c' m (sig', sig'') -> ds c m (sig, sig'').
+Proof.
+  intros m c sig c' sig' Hstep. induction Hstep; intros sig'' Hds.
+  - (* SAssign *) inversion Hds; subst. destruct m; simpl;
+      [ apply EDAssignV | apply EDAssignA ].
+  - (* SRand *) inversion Hds; subst. destruct m; simpl;
+      [ apply EDRandV | apply EDRandA ].
+  - (* SAssume *) inversion Hds; subst. apply EDAssume. exact H.
+  - (* SRead *) inversion Hds; subst. destruct m; simpl in *;
+      [ apply EDReadV | apply EDReadA ]; exact H.
+  - (* SWrite *) inversion Hds; subst. destruct m; simpl in *;
+      [ apply EDWriteV | apply EDWriteA ].
+  - (* SAdvAssertS *)
+    inversion Hds; subst; clear Hds. eauto using EDAdvAssertSuccess.
+  - (* SAdvAssertF *)
+    inversion Hds; subst; clear Hds. eauto using EDAdvAssertFailure.
+  - (* SSeqSkip *) eapply EDSeq. apply EDSkip. exact Hds.
+  - (* SSeqStep *) inversion Hds; subst.
+    eapply EDSeq; eauto.
+  - (* SChoiceL *) apply EDChoiceL. exact Hds.
+  - (* SChoiceR *) apply EDChoiceR. exact Hds.
+  - (* SStar0 *) inversion Hds; subst. apply EDStar0.
+  - (* SStarN *) inversion Hds; subst; eauto using ds_star_left.
+  - (* SLocalEnter *) apply ds_local_desugar. exact Hds.
+Qed.
+
+Lemma sstep_star_ds : forall m c sig c' sig',
+  sstep_star m c sig c' sig' ->
+  forall sig'', ds c' m (sig', sig'') -> ds c m (sig, sig'').
+Proof.
+  intros m c sig c' sig' H. induction H; intros sig0' Hds.
+  - exact Hds.
+  - eapply sstep_expansion. exact H. apply IHsstep_star. exact Hds.
+Qed.
+
+Theorem sstep_star_sound : forall m c sig sig',
+  sstep_star m c sig ASkip sig' -> ds c m (sig, sig').
+Proof.
+  intros m c sig sig' H. eapply sstep_star_ds. exact H. apply EDSkip.
+Qed.
+
+End Adequacy.
+
+(** Composed interleaving semantics *)
+Section ComposedInterleaving.
+
+Inductive cstep :
+  astmt -> astmt -> estate -> astmt -> astmt -> estate -> Prop :=
+| CStepP : forall cp ca cp' sig sig',
+    sstep Ok cp sig cp' sig' ->
+    cstep cp ca sig cp' ca sig'
+| CStepA : forall cp ca ca' sig sig',
+    sstep Ad ca sig ca' sig' ->
+    cstep cp ca sig cp ca' sig'
+| CStepComPA : forall cp ca (s : id) sig v l1 l2,
+    sig.(vstate).(ch) s = v :: l1 ->
+    sig.(astate).(ch) s = l2 ->
+    cstep cp ca sig cp ca
+          (sig[[ s :=vch l1 ]] [[ s :=ach (l2 ++ [v])%list ]])
+| CStepComAP : forall cp ca (s : id) sig v l1 l2,
+    sig.(astate).(ch) s = v :: l1 ->
+    sig.(vstate).(ch) s = l2 ->
+    cstep cp ca sig cp ca
+          (sig[[ s :=ach l1 ]] [[ s :=vch (l2 ++ [v])%list ]]).
+
+Inductive cstep_star :
+  astmt -> astmt -> estate -> astmt -> astmt -> estate -> Prop :=
+| CST0 : forall cp ca sig, cstep_star cp ca sig cp ca sig
+| CSTN : forall cp ca sig cp' ca' sig' cp'' ca'' sig'',
+    cstep cp ca sig cp' ca' sig' ->
+    cstep_star cp' ca' sig' cp'' ca'' sig'' ->
+    cstep_star cp ca sig cp'' ca'' sig''.
+
+Lemma cstep_star_trans : forall cp1 ca1 s1 cp2 ca2 s2 cp3 ca3 s3,
+  cstep_star cp1 ca1 s1 cp2 ca2 s2 ->
+  cstep_star cp2 ca2 s2 cp3 ca3 s3 ->
+  cstep_star cp1 ca1 s1 cp3 ca3 s3.
+Proof.
+  intros. induction H.
+  - assumption.
+  - eapply CSTN. exact H. apply IHcstep_star. assumption.
+Qed.
+
+(* Lift a single-threaded small-step run into the composed relation *)
+Lemma cstep_star_progL : forall cp ca sig cp' sig',
+  sstep_star Ok cp sig cp' sig' ->
+  cstep_star cp ca sig cp' ca sig'.
+Proof.
+  intros cp ca sig cp' sig' H. induction H.
+  - apply CST0.
+  - eapply CSTN. apply CStepP. exact H. exact IHsstep_star.
+Qed.
+
+Lemma cstep_star_progR : forall cp ca sig ca' sig',
+  sstep_star Ad ca sig ca' sig' ->
+  cstep_star cp ca sig cp ca' sig'.
+Proof.
+  intros cp ca sig ca' sig' H. induction H.
+  - apply CST0.
+  - eapply CSTN. apply CStepA. exact H. exact IHsstep_star.
+Qed.
+
+(** An attack is a terminating composed run that ends with both
+    sides finished and the adversary's assertion satisfied. *)
+Definition attack_reaches (cp ca : astmt) (sig0 : estate) (Post : aprop) : Prop :=
+  exists sigf, cstep_star cp ca sig0 ASkip ASkip sigf /\ Post sigf.
+
+(** [attack_reaches] for a full run of a multi-threaded system *)
+Definition attack_reaches_AL (m1 m2 : mode) (sp0 sa0 : estate) (Post : aprop) : Prop :=
+  exists sq sb, cds_star_hetero m1 m2 (sp0, sa0) (sq, sb) /\ Post sb.
+
+End ComposedInterleaving.
+
+Lemma sstep_star_under_seq : forall m c1 sig c1' sig' c2,
+  sstep_star m c1 sig c1' sig' ->
+  sstep_star m (ASeq c1 c2) sig (ASeq c1' c2) sig'.
+Proof.
+  intros m c1 sig c1' sig' c2 H. induction H.
+  - apply SS0.
+  - eapply SSN. apply SSeqStep. exact H. exact IHsstep_star.
+Qed.
+
+Lemma sstep_seq_run : forall m c1 sig sig' c2,
+  sstep_star m c1 sig ASkip sig' ->
+  sstep_star m (ASeq c1 c2) sig c2 sig'.
+Proof.
+  intros m c1 sig sig' c2 H.
+  eapply sstep_star_trans.
+  - apply (sstep_star_under_seq m c1 sig ASkip sig' c2). exact H.
+  - eapply SSN. apply SSeqSkip. apply SS0.
+Qed.
+
+Lemma sstep_one : forall m c sig sig',
+  sstep m c sig ASkip sig' -> sstep_star m c sig ASkip sig'.
+Proof. intros. eapply SSN. exact H. apply SS0. Qed.
+
+End SmallStepSemantics.
