theories/AL/language.v
@@ -70,19 +70,18 @@ Inductive astmt : Type :=
   | ARead (s x : id)
   | AWrite (s x : id)
   | AAdvAssert (P : prop)
-  | ACom (c1 c2 : astmt).
+  | ACom (c1 c2 : astmt)
+  | ALocal (x : id) (e : expression) (c : astmt).
 
 Open Scope al_scope.
 
 Notation "<{ e }>" := e (e custom al_stmt_aux) : al_scope.
-Notation "e" := e (in custom al_stmt_aux at level 0, e custom al_stmt) : al_scope.
-Notation "x" := x (in custom al_stmt at level 0, x constr at level 0) : al_scope.
-Notation "( x )" := x (in custom al_stmt, x at level 99) : al_scope.
-(* Notation "f x .. y" := (.. (f x) .. y)
-                  (in custom al_stmt at level 0, only parsing,
-                  f constr at level 0, x constr at level 9,
-                  y constr at level 9) : al_scope. *)
-(* Notation "'fun' s '=>' e" := (fun s => e) (in custom al_stmt at level 0, only parsing, s constr, e constr) : al_scope. *)
+Notation "e" := e
+  (in custom al_stmt_aux at level 0, e custom al_stmt) : al_scope.
+Notation "x" := x
+  (in custom al_stmt at level 0, x constr at level 0) : al_scope.
+Notation "( x )" := x
+  (in custom al_stmt, x at level 99) : al_scope.
 
 Notation "'skip'" := ASkip
   (in custom al_stmt at level 0) : al_scope.
@@ -122,6 +121,11 @@ Notation "'Com(' c1 ',' c2 ')'" := (ACom c1 c2)
    c1 custom al_stmt at level 99,
    c2 custom al_stmt at level 99, no associativity) : al_scope.
 
+Notation "'local' x '=' e 'in' c" := (ALocal x e c)
+  (in custom al_stmt at level 0,
+   x constr at level 0, e constr at level 85,
+   c custom al_stmt at level 99, no associativity) : al_scope.
+
 Declare Scope prop_scope.
 Bind Scope prop_scope with prop.
 Delimit Scope prop_scope with prop.
@@ -135,7 +139,7 @@ Notation "P ->> Q" := (aprop_impl P Q) (at level 80).
 
 Notation assert P := (P%prop : aprop).
 
-Notation "~ P" := (fun st => ~ assert P st) (in custom al_stmt at level 0) : prop_scope.
+Notation "~ P" := (fun st => ~ assert P st) (in custom al_stmt at level 0, P constr at level 0) : prop_scope.
 Notation "P /\ Q" := (fun st => assert P st /\ assert Q st) : prop_scope.
 Notation "P \/ Q" := (fun st => assert P st \/ assert Q st) : prop_scope.
 Notation "P -> Q" := (fun st => assert P st -> assert Q st) : prop_scope.
